Aesop/Builder/Unfold.lean
@@ -32,8 +32,9 @@ def checkUnfoldableConst (decl : Name) : MetaM (Option Name) :=
           throwError "Recursive definition '{decl}' cannot be used as an unfold rule (it would be unfolded infinitely often). Try adding a simp rule for it."
     return unfoldThm?
 
+-- TODO support local unfold rules
 def unfold : RuleBuilder := λ input => do
-  let decl ← resolveConstRuleName input.ident .unfold
+  let decl ← elabGlobalRuleIdent .unfold input.term
   let unfoldThm? ← checkUnfoldableConst decl
   return .global $ .base $ .unfoldRule { decl, unfoldThm? }
 
