AesopTest/CompositeLocalRuleTerm.lean
@@ -1,0 +1,50 @@
+/-
+Copyright (c) 2024 Jannis Limperg. All rights reserved.
+Released under Apache 2.0 license as described in the file LICENSE.
+Authors: Jannis Limperg
+-/
+
+import Aesop
+import Std.Tactic.GuardMsgs
+
+set_option aesop.check.all true
+set_option aesop.smallErrorMessages true
+
+-- Composite terms are supported by the `apply` and `forward` builders...
+
+structure A where
+
+/--
+error: tactic 'aesop' failed, made no progress
+-/
+#guard_msgs in
+example (h : A → β → γ) (b : β) : γ := by
+  aesop
+
+example (h : A → β → γ) (b : β) : γ := by
+  aesop (add safe apply (h {}))
+
+example (h : A → β → γ) (b : β) : γ := by
+  aesop (add safe forward (h {}))
+
+-- ... and also by the `simp` builder.
+
+/--
+error: tactic 'aesop' failed, made no progress
+-/
+#guard_msgs in
+example {P : α → Prop} (h : A → x = y) (p : P x) : P y := by
+  aesop
+
+example {P : α → Prop} (h : A → x = y) (p : P x) : P y := by
+  aesop (add simp (h {}))
+
+/--
+error: tactic 'aesop' failed, made no progress
+-/
+#guard_msgs in
+example {P : α → Prop} (h₁ : A → x = y) (h₂ : A → y = z) (p : P x) : P z := by
+  aesop
+
+example {P : α → Prop} (h₁ : A → x = y) (h₂ : A → y = z) (p : P x) : P z := by
+  aesop (add simp [(h₁ {}), (h₂ {})])
